Prefix.v
@@ -12,6 +12,8 @@ Section PREFIX.
 
 Definition B: Type := list bool.
 
+(* note all of this prefix stuff doesn't require B to be a list of bool;
+it could be any type with decidable equality. *)
 (* is b1 a prefix of b2 *)
 Fixpoint is_prefix_bool (b1 b2: B): bool :=
   match b1 with
@@ -82,15 +84,102 @@ Proof.
 induction b; autounfold; simpl; intros; trivial.
 discriminate.
 Qed.
+
 (*
-Lemma is_prefix_append: forall p b f, is_prefix p (b ++ (f::nil)) ->
+Lemma list_induction_append: forall T P,
+  P nil ->
+  (forall l (v: T), P l -> P (l ++ (v::nil))) ->
+  (forall l, P l).
+Proof.
+Qed.*)
+
+(*
+Lemma nonempty_append: forall T l (v: T),
+  exists s, cons v l = (firstn (length l) (cons v l)) ++ s::nil.
+Proof.
+induction l; simpl; intros.
+- exists v. reflexivity.
+-  
+
+Qed.*)
+
+Lemma nonzero_length: forall T (l: list T),
+  l <> nil <-> 1 <= length l.
+Proof.
+destruct l; simpl.
+- split; intro. contradiction. omega.
+- split; intro. omega. intro. discriminate.
+Qed.
+
+Lemma apply_both_sides: forall T U (f: T->U) a b,
+  a = b -> f a = f b.
+Proof.
+intros. rewrite H. reflexivity.
+Qed.
+
+Lemma removelast_both_sides: forall T (a: list T) b,
+  a = b -> removelast a = removelast b.
+Proof.
+intros. apply apply_both_sides. assumption.
+Qed.
+
+Lemma length_both_sides: forall T (a: list T) b,
+  a = b -> length a = length b.
+Proof.
+intros. apply apply_both_sides. assumption.
+Qed.
+
+(* docs say this is in the List library, but it's not there.
+so we prove it.
+*)
+Lemma removelast_last:
+  forall T l (a: T), removelast (l ++ a::nil) = l.
+Proof.
+induction l; simpl; intros.
+reflexivity.
+remember (l ++ a0::nil) as l0. destruct l0.
+- apply length_both_sides in Heql0.
+rewrite app_length in Heql0. simpl in Heql0. omega.
+-
+apply removelast_both_sides in Heql0.
+rewrite IHl in Heql0. rewrite Heql0. reflexivity.
+Qed.
+
+Lemma append_nonempty_prefix: forall p b x f,
+  p ++ x = b ++ (f::nil) ->
+  1 <= length x ->
+  is_prefix p b.
+Proof.
+intros. apply is_prefix_app.
+apply nonzero_length in H0.
+destruct (exists_last H0). destruct s.
+subst x.
+exists x0.
+apply removelast_both_sides in H.
+rewrite app_assoc in H.
+repeat rewrite removelast_last in H.
+assumption.
+Qed.
+
+(*
+it's true but hard to prove
+Lemma prefix_length: forall p b x y,
+  p ++ x = b ++ y ->
+  length y <= length x ->
+  is_prefix p b.
+Proof.
+*)
+
+Lemma is_prefix_append: forall p b f,
+  is_prefix p (b ++ (f::nil)) ->
   is_prefix p b \/ p = b ++ (f::nil).
 Proof.
 intros. apply is_prefix_app in H. 
 destruct H.
 rewrite <- H. destruct x.
 - right. rewrite app_nil_r. reflexivity.
-- left. apply is_prefix_spec.
+- left. apply append_nonempty_prefix in H. assumption.
+simpl. omega.
 Qed.
-*)
+
 End PREFIX.
